@prefix : <https://w3id.org/pmd/hmo/> .
@prefix pmdco: <https://w3id.org/pmd/co/> .
@prefix owl: <http://www.w3.org/2002/07/owl#> .
@prefix rdf: <http://www.w3.org/1999/02/22-rdf-syntax-ns#> .
@prefix xml: <http://www.w3.org/XML/1998/namespace> .
@prefix xsd: <http://www.w3.org/2001/XMLSchema#> .
@prefix rdfs: <http://www.w3.org/2000/01/rdf-schema#> .
@base <https://w3id.org/pmd/hmo> .

<https://w3id.org/pmd/hmo> rdf:type owl:Ontology ;
                            owl:imports <https://w3id.org/pmd/co> ;
                            #<http://purl.org/dc/elements/1.1/creator> <https://orcid.org/0000-0001-7192-7143> ,
                            #                                          <https://orcid.org/0000-0002-3717-7104> ,
                            #                                          <https://orcid.org/0000-0002-7094-5371> ,
                            #                                          <https://orcid.org/0000-0002-9014-2920> ,
                            #                                          <https://orcid.org/0000-0003-4971-3645> ;
                            <http://purl.org/dc/elements/1.1/license> <http://creativecommons.org/licenses/by/4.0/> ;
                            #<http://purl.org/dc/terms/bibliographicCitation> "Markus Schilling, Bernd Bayerlein, Henk Birkholz, Philipp von Hartrott, Jörg Waitelonis. (August 1st, 2023) TTO: Tensile Test Ontology. Version 2.0.2, https://w3id.org/pmd/co"@en ;
                            <http://purl.org/dc/terms/created> "2023-08-18"@en ;
                            <http://purl.org/dc/terms/title> "Hardness Measurement Ontology (HMO)"@en ;
                            owl:versionInfo "0.0.1" ;
                            <http://www.w3.org/2004/02/skos/core#definition> """This is the development version of the PMD ontology module of hardness measurements (Hardness Measurement Ontology - HTO) as developed on the basis of the standard ISO 6507-1: Metallic materials - Vickers hardness test - Part 1: Test method.

The HMO was developed in the frame of the PMD project. The HMO provides conceptualizations valid for the description of Vickers hardness test and corresponding data in accordance with the respective standard. By using HMO for storing vickers hardness test data, all data will be well structured and based on a common vocabulary agreed on by an expert group (generation of FAIR data) which will lead to enhanced data interoperability. This comprises several data categories such as primary data, secondary data and metadata. Data will be human and machine readable. The usage of HMO facilitates data retrieval and downstream usage. Due to a close connection to the mid-level PMD core ontology (PMDco), the interoperability of hardness test data is enhanced and querying in combination with other aspects and data within the broad field of material science and engineering (MSE) is facilitated.

The HMO class structure forms a comprehensible and semantic layer for unified storage of data generated in a hardness test including the possibility to record data from analysis, re-evaluation and re-use. Furthermore, extensive metadata allows to assess data quality and reproduce experiments. Following the open world assumption, object properties are deliberately low restrictive and sparse.

HMO of PMD at GitHub: https://github.com/materialdigital/application-ontologies/tree/main/tensile_test_ontology_TTO"""@en ;
                            <http://www.w3.org/ns/prov#editorialNote> "The tensile test ontology (HMO) was developed in the frame of the joint project of platform material digital (PMD). As being one of the modules of it, the HMO is strongly connected to the PMD core ontology (PMDco) and thus, HMO concepts use the namespace https://w3id.org/pmd/co."@en .

#################################################################
#    Object Properties
#################################################################

###  https://w3id.org/pmd/hmo/relatesToExtension
#:relatesToExtension rdf:type owl:ObjectProperty ;
#                    rdfs:subPropertyOf :relatesTo ;
#                    rdfs:domain :ProofStrengthPlasticExtension ;
#                    rdfs:range :PercentageExtension ;
#                    rdfs:isDefinedBy <https://w3id.org/pmd/tto> ;
#                    rdfs:label "relates to extension"@en .


#################################################################
#    Classes
#################################################################

###  https://w3id.org/pmd/co/ISO6507-1VickersHardnessTest
:ISO6507-1VickersHardnessTest rdf:type owl:Class ;
                             owl:equivalentClass [ rdf:type owl:Restriction ;
                                                   owl:onProperty pmdco:participant ;
                                                   owl:someValuesFrom :VickersHardnessTestingMachine
                                                 ] ,
                                                 [ rdf:type owl:Restriction ;
                                                   owl:onProperty pmdco:participant ;
                                                   owl:someValuesFrom :VickersIndenter
                                                 ] ,
                                                 [ rdf:type owl:Restriction ;
                                                   owl:onProperty pmdco:participant ;
                                                   owl:someValuesFrom :DiagonalMeasuringSystem
                                                 ] ,
                                                 [ rdf:type owl:Restriction ;
                                                   owl:onProperty pmdco:participant ;
                                                   owl:someValuesFrom pmdco:TestPiece
                                                 ] ,
                                                 [ rdf:type owl:Restriction ;
                                                   owl:onProperty pmdco:characteristic ;
                                                   owl:someValuesFrom :VickersTestForce
                                                 ] ;
                             rdfs:subClassOf pmdco:MechanicalTestingProcess ;
                             rdfs:isDefinedBy <https://w3id.org/pmd/hmo> ;
                             rdfs:label "Vickers hardness test in accordance with ISO 6507-1"@en ,
                                        "Vickers-Härtemessung nach ISO 6507-1"@de ;
                             #<http://www.w3.org/2004/02/skos/core#definition> "Dieses Wertobjekt beschreibt eine Variation der Abmessungen eines Prüfkörpers in Bezug auf seine Querachse, die sich auf seine Querschnittsfläche auswirkt und möglicherweise während eines Zugversuchs auftritt. Das Verhältnis der wahren plastischen Breitendehnung und der wahren plastischen Dickendehnung in einem in uniaxialem Zug beanspruchten Prüfkörper (vertikale Anisotropie) kann anhand dieser Information berechnet werden."@de ,
                             #                                                 "This value object describes a variation in the dimension of a test piece referring to its transversal axis affecting its cross-sectional area that may potentially occur during a tensile test. The ratio of the true plastic strain in width and the true plastic strain in thickness in a test piece loaded in uniaxial tension (vertical anisotropy) may be calculated using this information."@en ;
                             pmdco:definitionSource "DIN EN ISO 6507-1:2018-07" .


###  https://w3id.org/pmd/co/VickersHardnessTestingMachine
:VickersHardnessTestingMachine rdf:type owl:Class ;
                             rdfs:subClassOf pmdco:TestingMachine ;
                             rdfs:isDefinedBy <https://w3id.org/pmd/hmo> ;
                             rdfs:label "Testing machine for the Vickers hardness test in accordance with ISO 6507-2"@en ,
                                        "Prüfmaschine für die Vickers-Härtemessung in Übereinstimmung mit ISO 6507-2"@de ;
                             #<http://www.w3.org/2004/02/skos/core#definition> "Dieses Wertobjekt beschreibt eine Variation der Abmessungen eines Prüfkörpers in Bezug auf seine Querachse, die sich auf seine Querschnittsfläche auswirkt und möglicherweise während eines Zugversuchs auftritt. Das Verhältnis der wahren plastischen Breitendehnung und der wahren plastischen Dickendehnung in einem in uniaxialem Zug beanspruchten Prüfkörper (vertikale Anisotropie) kann anhand dieser Information berechnet werden."@de ,
                             #                                                 "This value object describes a variation in the dimension of a test piece referring to its transversal axis affecting its cross-sectional area that may potentially occur during a tensile test. The ratio of the true plastic strain in width and the true plastic strain in thickness in a test piece loaded in uniaxial tension (vertical anisotropy) may be calculated using this information."@en ;
                             pmdco:definitionSource "DIN EN ISO 6507-1:2018-07" .


###  https://w3id.org/pmd/co/VickersIndenter
:VickersIndenter rdf:type owl:Class ;
                     rdfs:subClassOf pmdco:Component ;
                     rdfs:isDefinedBy <https://w3id.org/pmd/hmo> ;
                     rdfs:label "Indenter for the Vickers hardness measurement as specified in ISO 6507-2"@en ,
                                "Eindringkörper für die Vickers-Härtemessung nach ISO 6507-2"@de ;
                     #<http://www.w3.org/2004/02/skos/core#definition> "Diese Eigenschaft beschreibt die Verschiebung der Traverse einer Zugprüfmaschine."@de ,
                     #                                                 """Dimensional analysis: L
Unit (e.g. SI): mm"""@en ,
                     #                                                 "This property describes the displacement of the crossheads of a tensile testing machine."@en ;
                     pmdco:definitionSource "DIN EN ISO 6507-1:2018-07"@en .


###  https://w3id.org/pmd/co/DiagonalMeasuringSystem
:DiagonalMeasuringSystem rdf:type owl:Class ;
                     rdfs:subClassOf pmdco:MeasuringDevice ;
                     rdfs:isDefinedBy <https://w3id.org/pmd/hmo> ;
                     rdfs:label "Diagonal measuring system for the Vickers hardness measurement as specified in ISO 6507-2"@en ,
                                "Diagonalmesssystem für die Vickers-Härtemessung nach ISO 6507-2"@de ;
                     #<http://www.w3.org/2004/02/skos/core#definition> "Diese Eigenschaft beschreibt die Verschiebung der Traverse einer Zugprüfmaschine."@de ,
                     #                                                 """Dimensional analysis: L
Unit (e.g. SI): mm"""@en ,
                     #                                                 "This property describes the displacement of the crossheads of a tensile testing machine."@en ;
                     pmdco:definitionSource "DIN EN ISO 6507-1:2018-07"@en .


###  https://w3id.org/pmd/co/VickersTestForce
:VickersTestForce rdf:type owl:Class ;
                     rdf:subClassOf pmdco:SetPoint ;
                     rdf:subClassOf pmdco:PrimaryData ; ##TODO: Macht das so Sinn?
                     rdfs:subClassOf pmdco:Force ;
                     rdfs:isDefinedBy <https://w3id.org/pmd/hmo> ;
                     rdfs:label "Test force used in the Vickers hardness measurement"@en ,
                                "Prüfkraft, die für die Vickers-Härtemessung verwendet wurde"@de ;
                     #<http://www.w3.org/2004/02/skos/core#definition> "Diese Eigenschaft beschreibt die Verschiebung der Traverse einer Zugprüfmaschine."@de ,
                     #                                                 """Dimensional analysis: L
Unit (e.g. SI): mm"""@en ,
                     #                                                 "This property describes the displacement of the crossheads of a tensile testing machine."@en ;
                     pmdco:definitionSource "DIN EN ISO 6507-1:2018-07"@en .


###  https://w3id.org/pmd/co/VickersTestForceDuration
:VickersTestForce rdf:type owl:Class ;
                     rdf:subClassOf pmdco:SetPoint ;
                     rdf:subClassOf pmdco:PrimaryData ; ##TODO: Macht das so Sinn?
                     rdfs:subClassOf pmdco:Duration ;
                     rdfs:isDefinedBy <https://w3id.org/pmd/hmo> ;
                     rdfs:label "Test force used in the Vickers hardness measurement"@en ,
                                "Prüfkraft, die für die Vickers-Härtemessung verwendet wurde"@de ;
                     #<http://www.w3.org/2004/02/skos/core#definition> "Diese Eigenschaft beschreibt die Verschiebung der Traverse einer Zugprüfmaschine."@de ,
                     #                                                 """Dimensional analysis: L
Unit (e.g. SI): mm"""@en ,
                     #                                                 "This property describes the displacement of the crossheads of a tensile testing machine."@en ;
                     pmdco:definitionSource "DIN EN ISO 6507-1:2018-07"@en .


###  Generated by the OWL API (version 4.5.9.2019-02-01T07:24:44Z) https://github.com/owlcs/owlapi
